code/rocq/wip/valid_state.v
@@ -1,0 +1,728 @@
+From mathcomp Require Import all_ssreflect.
+From det Require Import lang.
+
+Module valid_state (U:Unif).
+  Module Run := Run(U).
+  Include Run.
+  
+  Fixpoint base_and s :=
+    match s with
+    | And (Goal _ _) r r1 => (r == r1) && base_and r1 (* should also say something about the program *)
+    | Top => true
+    | _ => false
+    end.
+
+  Lemma base_and_dead {A}: base_and (dead A) = false.
+  Proof. case: A => // -[]//=. Qed.
+
+  Fixpoint base_or_aux s :=
+    match s with
+    | Or l _ r => base_and l && (base_or_aux r) (* todo: should also say something about the substitution and the program? *)
+    | t => base_and t
+    end.
+
+  Definition base_or s := 
+    match s with 
+    | Bot => true
+    | Or Bot _ t => base_or_aux t
+    | _ => false
+    end.
+
+  Fixpoint base_and_ko s :=
+    match s with
+    | And KO r r1 => [&&base_and r, (cut r == r1) & base_and_ko r1] (* should also say something about the program *)
+    | KO => true
+    | _ => false
+    end.
+
+  Fixpoint base_or_aux_ko s :=
+    match s with
+    | Or l _ r => base_and_ko l && (base_or_aux_ko r) (* todo: should also say something about the substitution and the program? *)
+    | t => base_and_ko t
+    end.
+
+  Lemma base_and_big_and {pr A}: base_and (big_and pr A).
+  Proof. by elim: A => // a l /= ->; rewrite eq_refl. Qed.
+
+  (* same_structure_and *)
+  Section ssa.
+    Fixpoint ssa A B :=
+      match A, B with
+      | And _ _ _, Or _ _ _ => false
+      | And _ _ A, And _ _ B => ssa A B
+      | Top, (Top|OK|KO|Dead) => true
+      | _, _ => false
+      end.
+
+    Lemma xxx {B C D}: base_and B -> base_and D -> ssa B C -> ssa D C -> ssa B D.
+    Proof.
+      elim: B C D => //.
+      + move=>[]//[]//=[]//.
+      + move=> []//p a _ A HA B HB[]//=C D E []//.
+        move=> []///= _ _ F G.
+        move=>/andP[]/eqP <- bA /andP[]/eqP? ssA ssF.
+        apply: HA => //.
+    Qed.
+
+
+    Lemma ssa_id {A}: base_and A -> ssa A A.
+    Proof. by elim: A =>// -[]// p a _ B0 HB0 B HB/=/andP[] _. Qed.
+
+    Lemma ssa_cut {A}: base_and A -> ssa A (cut A).
+    Proof. by elim: A =>// -[]// p a _ B0 HB0 B HB/=/andP[] _. Qed.
+
+    Lemma ssa_dead {A}: base_and A -> ssa A (dead A).
+    Proof. elim: A =>//= -[]// p a _ B0 HB0 B HB/=/andP[] _//. Qed.
+
+    Lemma ssa_cut1 {A B}: ssa A B -> ssa A (cut B).
+    Proof.
+      elim: A B; try by move=> // [] //.
+      - move=> A HA B0 _ B HB[]//.
+    Qed.
+
+    Lemma ssa_dead1 {A B}: ssa A B -> ssa A (dead B).
+    Proof.
+      elim: A B; try by move=> // [] //.
+      - move=> A HA B0 _ B HB[]//.
+    Qed.
+
+    Lemma ssa_cut2 {A B}: base_and B -> ssa A (cut B) -> ssa A B.
+    Proof.
+      elim: A B; try by move=> []//.
+      (* - move=> /= _ _ []//.
+      - move=> A HA s B HB []//. *)
+      - move=> A HA B0 _ B HB[]//[]//.
+        move=> p a s1 s2/=/andP[]/eqP?;subst.
+        apply: HB.
+    Qed.
+
+    (* Lemma xxx {B C D}: ssa B C -> ssa D C -> ssa B D.
+    Proof.
+      elim: B C D => //.
+      + move=>[]//[]//.
+      + move=> A HA B0 HB0 B HB[]//.
+          move=> [] //=. *)
+
+    Lemma ssa_expand {B0 B s r}: base_and B0 -> ssa B0 B -> expand s B = r -> ssa B0 (get_state r).
+    Proof.
+      elim: B0 B s r => //.
+        move=>[]//s []//.
+        - move=> ? _ _ [] <-//.
+        - move=> ?? _ _ [] <-//<-//.
+        - move=> ?? _ _ [] <-//<-//.
+        - move=> ? _ _ [] <-//.
+      move=> []// p a _ A HA B0 HB0 []// A' B0' B' s.
+      move=>/= r /andP[]/eqP? bB ssB0;subst.
+      case: r =>//.
+      + move=> s1 C /simpl_expand_and_expanded[].
+          move=>[A2[HA' ->]]//.
+        move=>[s' [A2 [B2 [HA' [HB' ->]]]]]//=.
+        by apply: HA _ _ _ bB _ HB'.
+      + move=> s1 C /simpl_expand_and_cut[].
+          move=>[A2 [HA' ->]]//.
+        move=> [s'[A2[B2 [HA'[HB' ->]]]]]/=.
+        by apply: HA _ _ _ bB _ HB'.
+      + move=> C /simpl_expand_and_fail[].
+          move=> [A2 [HA' ->]]//=.
+        move=>[s' [A2[B2 [HA' [HB' ->]]]]]//=.
+        by rewrite (HA _ _ _ bB ssB0 HB').
+      + move=> s1 C /simpl_expand_and_solved.
+        move=> [s'[A1[B1[HA'[HB' ->]]]]]/=.
+        by have /= := (HA _ _ _ bB ssB0 HB').
+    Qed.
+  End ssa.
+
+  
+  Fixpoint valid_state s :=
+    match s with
+    | Goal _ _ | OK | KO | Bot | Top => true
+    | Dead => false
+    | Or A _ B => 
+      if A == dead A then valid_state B
+      else valid_state A && (base_or_aux B || base_or_aux_ko B)
+    | And A B0 B => 
+      [&& valid_state A,
+        if success A then valid_state B 
+        else ((B0 == B) || (cut B0 == B)),
+        ssa B0 B &
+        (base_and B0)]
+    end.
+
+  Lemma valid_state_dead {A} : valid_state (dead A) = false.
+  Proof.
+    elim: A => //.
+      by move=> A HA s B HB/=; rewrite dead_dead_same eqxx.
+    move=> A HA Bo ? B HB/=.
+    rewrite HA//.
+  Qed.
+
+  Lemma base_and_valid {A} : base_and A -> valid_state A.
+  Proof.
+    elim A => //; clear => A HA B +; rewrite /base_or_aux //=; case: A HA => //.
+    move=> p a _ + A + /andP [] /eqP H ; rewrite H.
+    move=> _ HVA HA; rewrite (HVA HA) /=.
+    by rewrite HA eq_refl (ssa_id HA).
+  Qed.
+
+
+  Lemma valid_state_big_and {pr l} : valid_state (big_and pr l).
+  Proof.
+    elim: l => // x xs /=.
+    by rewrite base_and_big_and eq_refl/= (ssa_id base_and_big_and).
+  Qed.
+
+  Lemma base_or_big_and {pr l} : base_or_aux (big_and pr l).
+  Proof. case: l; rewrite /base_or_aux //= => ??; by rewrite base_and_big_and eqxx. Qed.
+
+  Lemma base_or_big_or_aux {pr s l}: base_or_aux (big_or_aux pr s l).
+  Proof.
+    elim: l s => //=; clear.
+    + move=> ?; apply: base_or_big_and.
+    + by move=> [[s r] rs] IH r1 /=; rewrite IH base_and_big_and.
+  Qed.
+
+  Lemma base_or_valid {A} : base_or_aux A -> valid_state A.
+  Proof.
+    elim A => //; clear.
+    + move=> A HA s B HB/=/andP[bA bB].
+      case:ifP => /eqP.
+        by move=>H; move: bA; rewrite H base_and_dead.
+      rewrite bB // base_and_valid//.
+    + move=> []// p a Ha B0 HB0 B HB /=/andP[/eqP->]bB.
+      by rewrite eqxx bB (ssa_id bB).
+  Qed.
+
+  Lemma simpl_valid_state_or {s A B}: 
+    valid_state (Or A s B) -> 
+      (A = dead A /\ valid_state B) \/ 
+      (A <> dead A /\ valid_state A /\ (base_or_aux B || base_or_aux_ko B)).
+  Proof.
+    move=> /=; case: A => //.
+    all: try by move=> /= ->; right; repeat split => //; rewrite orbT //.
+    + move=> /= ->; left => //.
+    + move=> ?? /orP [] ->; right; repeat split => //; rewrite orbT //.
+    + move=> ???; case:ifP=>/eqP//.
+        by move=>/=[]->->; rewrite !dead_dead_same eqxx; left.
+      move=> H/andP[]->->; auto.
+    + move=> ???; case:ifP=>/eqP.
+        move=>->->; rewrite dead_dead_same; auto.
+      move=>? /andP[]->->; auto.
+  Qed.
+
+  Lemma base_and_ko_valid {B}: base_and_ko B -> valid_state B.
+  Proof.
+    elim: B => //.
+    by move=> []// HA B0 _ B HB/=/and3P[bB0 /eqP <-]; rewrite bB0 eqxx orbT (ssa_cut bB0).
+  Qed.
+
+  Lemma simpl_valid_state_and1 {A B0 B}: valid_state (And A B0 B) -> 
+    valid_state A /\ 
+      ( 
+        (* if A == dead A then B == dead B else  *)
+        if success A then valid_state B 
+        else ((B0 == B) || (cut B0 == B))) 
+      /\ ssa B0 B /\ base_and B0.
+  Proof. by move=>/=/and3P[]//->->/andP[]->->. Qed.
+
+
+  Lemma base_or_ko_valid {B}: base_or_aux_ko B -> valid_state B.
+  Proof.
+    elim: B => //.
+    + move=> A HA s B HB /= /andP [] /base_and_ko_valid ->.
+      move=> /[dup] /HB -> ->.
+      by rewrite orbT if_same.
+    + by move=> [] // HA B0 _ B HB /= /and3P[] bB0 /eqP <-; rewrite eq_refl bB0 orbT (ssa_cut bB0).
+  Qed.
+
+
+  Lemma base_or_base_or_ko_valid {B}:
+    base_or_aux B || base_or_aux_ko B -> valid_state B.
+  Proof. by move=> /orP []; [move=> /base_or_valid | move=> /base_or_ko_valid] => ->. Qed.
+
+
+  Lemma base_and_base_and_ko_cut {B} : base_and B -> base_and_ko (cut B).
+  Proof. 
+    elim: B => // A + B + C /=.
+    case: A => //= _ _ _ HB HC /andP [] /eqP <- hB.
+    by rewrite hB (HB hB) eqxx.
+  Qed.
+
+  Lemma base_or_base_or_ko_cut {B}: base_or_aux B -> base_or_aux_ko (cut B).
+  Proof.
+    elim: B => //.
+    + by move=> A IHA s B IHB /= /andP [] /base_and_base_and_ko_cut -> /IHB ->.
+    + move=> [] //= _ _ _ B HB C HC /andP [] /eqP /[subst1] hC.
+      by rewrite eq_refl hC (base_and_base_and_ko_cut hC). 
+  Qed.
+
+  Lemma base_and_ko_cut {B}: base_and_ko B -> base_and_ko (cut B).
+  Proof.
+    elim: B => //.
+    move=> []// _ B _ C HC /= /and3P[] bB /eqP <-.
+    by rewrite cut_cut_same eqxx bB => ->.
+  Qed.
+  
+  Lemma base_or_ko_cut {B}: base_or_aux_ko B -> base_or_aux_ko (cut B).
+  Proof.
+    elim: B => //.
+      by move=> A HA s B HB /= /andP[]/base_and_ko_cut->/HB->.
+    move=> [] //= _ B0 _ B HB /and3P[] bB /eqP<-.
+    by rewrite cut_cut_same bB eqxx => ->.
+  Qed.
+
+  Lemma cut_dead1 {A}: cut A = dead A -> dead A = A.
+  Proof. 
+    elim: A=> //.
+      move=> A HA s B HB/=[]??; rewrite HA//HB//.
+    move=> A HA B0 _ B HB/=[]??; rewrite HA//HB//.
+  Qed.
+
+  Lemma success_cut {A} : success (cut A) = success A.
+  Proof.
+    elim: A => //. 
+    + move=> A HA s B HB /=.
+      rewrite dead_cut_is_dead.
+      case:ifP=>/eqP.
+        by move=> /cut_dead1//->; rewrite eqxx.
+      by case: eqP => //->; rewrite dead_dead_same cut_dead_is_dead.
+    + move=> A HA B HB C HC /=.
+      by rewrite HA HC.
+  Qed.
+
+  Lemma valid_state_cut {A}: valid_state A -> valid_state (cut A).
+  Proof.
+    elim: A => //.
+      move=> A HA s B HB/simpl_valid_state_or[].
+        by move=>[]/=->; rewrite cut_dead_is_dead dead_dead_same eqxx.
+      move=> [DA[VA bB]]/=.
+      rewrite (HA VA) (HB (base_or_base_or_ko_valid bB)).
+      by move: bB => /orP[/base_or_base_or_ko_cut | /base_or_ko_cut]->; rewrite !orbT if_same.
+    move=> A HA B0 _ B HB /=/simpl_valid_state_and1[VA [+ [ssaB0 bB0]]].
+    rewrite (HA VA) success_cut bB0 andbT/=.
+    case: ifP => sA.
+      (* move=>->/eqP->; rewrite !cut_dead_is_dead !dead_dead_same !eqxx ssa_dead1//. *)
+    (* move=> dA; case: ifP => sA. *)
+      move=>vB; rewrite HB//ssa_cut1//.
+    move=> /orP[|]/eqP<-; rewrite ?cut_cut_same ?cut_dead_is_dead eqxx !orbT ?ssa_cut//.
+  Qed.
+
+  Lemma valid_state_compose_and {A2 B2 B02}: 
+    (if success A2 then valid_state B2 else ((B02 == B2) || (cut B02 == B2))) ->
+      base_and B02  ->
+        valid_state B2.
+  Proof. 
+    case: success => //.
+    move=>/orP[].
+      move=>/eqP->; apply: base_and_valid.
+    move=>/eqP<-/base_and_valid;apply: valid_state_cut.
+  Qed.
+
+  Lemma simpl_valid_state_and {A B0 B}: valid_state (And A B0 B) -> 
+    valid_state A /\ valid_state B.
+  Proof.
+    move=>/= /and3P[]// -> VB /andP[ssB0 bbB0].
+    by rewrite (valid_state_compose_and VB bbB0).
+  Qed.
+
+  (* Lemma expand_failure_dead s1 {A}: valid_state A -> expand s1 A <> Failure Dead.
+  Proof.
+    elim: A s1 => //.
+    + move=> /= p [] //.
+    + move=> A HA s B HB s1 /simpl_valid_state_or[].
+        by move=> [] ->/=/(HB s1) ; case X: expand => //= [[]]//.
+      move=>[] DA[]/HA{}HA/base_or_base_or_ko_valid/HB{}HB.
+      move=> /simpl_expand_or_fail[].
+        by move=> [? []] + []//.
+      move=> [].
+        by move=> []+[]+[]+[]//.
+      by move=> []+[]//; have:= (HA s1).
+    + move=> A HA B0 _ B HB s1 /simpl_valid_state_and[VA VB].
+      move=>/simpl_expand_and_fail[].
+        by move=>[]; have:= HA s1 VA.
+      move=> [].
+        by move=> []+[]+[]//.
+      move=> []s'[]A'[]B'[]H1[]H2.
+      case: eqP => ///[subst1].
+      by have:= HB s' VB.
+    Qed. *)
+
+  Lemma valid_state_big_or {pr s t} : valid_state (big_or pr s t).
+  Proof.
+    case: t; rewrite /big_or//=.
+    + by move=> ?; case: F => //= -[] //=???; rewrite base_or_big_or_aux.
+    + by move=> ?; case: F => //= -[] //=???; rewrite base_or_big_or_aux.
+    + by move=> ??; case F => //= -[] //=???; rewrite base_or_big_or_aux.
+  Qed.   
+
+  Lemma expand_not_dead {s A r}: 
+    valid_state A -> expand s A = r -> get_state r <> dead (get_state r) .
+  Proof.
+    elim: A s r; try by move=> //= _ r _ <-//.
+    + move=> p [|t] s r _ <- //= /esym; apply dead_big_or.
+    + move=> A HA s B HB s1 => // C /simpl_valid_state_or [].
+        move=> []->/= VB <-.
+        rewrite dead_dead_same eqxx.
+        have {}HB:= HB _ _ VB.
+        case X: expand => //=; have:= HB _ _ X => /=; try congruence.
+        (* by move=> H; case: ifP => /eqP H1; subst => //= -[]//. *)
+      move=> [DA[VA VB]].
+      case: C.
+      + move=> s2 C /simpl_expand_or_expanded [].
+          move=> [A'[DA'[HA' ->]]]/=[].
+          by have /= := HA _ _ VA HA'.
+        move=> [].
+          move=> [A'[dA []]] /HA => /(_ VA)/= HA' -> /=; rewrite dead_cut_is_dead; congruence.
+        move=>  [->[B' [H]]]->/=.
+        rewrite dead_dead_same => -[].
+        by move: H => []/HB/=/(_ (base_or_base_or_ko_valid VB))//.
+      + move=> s2 C /simpl_expand_or_cut [s3[B'[?]]]; subst => //.
+      + move=> C /simpl_expand_or_fail[].
+          move=>[A'[dA[HA']]]/=->.
+          have:= HA _ _ VA HA' => /=; congruence.
+        by move=>[B'[X]]; move: VA; rewrite X valid_state_dead.
+      + move=> s2 C /simpl_expand_or_solved [].
+          move=> [A'[]] /HA{} => /(_ VA) /= H ->/=; congruence.
+        move=> [B'[HA'[]]] /HB => /(_ (base_or_base_or_ko_valid VB)) /= + ->/=; congruence.
+    + move=> A HA B0 HB0 B HB s1 r /simpl_valid_state_and[] VA VB.
+      case: r.
+      + move=> s2 C /simpl_expand_and_expanded [].
+          by move=> [A'][] /HA => /(_ VA) /= ? ->[].
+        by move=> [s'[A'[B'[]]]] /HA /= +[] _ ->//= => /(_ VA) + [].
+      + move=> s2 C /simpl_expand_and_cut [].
+          by move=> [A'][] /HA /= + ->// => /(_ VA) + [].
+        move=> [s'[A'[B'[]]]] /HA/= + [] _->// => /(_ VA) + [].
+        rewrite dead_cut_is_dead => H /cut_dead1; congruence.
+      + move=> C /simpl_expand_and_fail [].
+          by move=>[A'[H ->]]/=[]; have:= (HA _ _ VA H).
+        move=>[s'[A'[B'[HA'[HB' ->]]]]]/=[].
+        by have:= HA _ _ VA HA'.
+      + move=> s2 C /simpl_expand_and_solved [s'[A'[B'[HA'[HB'->]]]]]/=[].
+        by have:= HA _ _ VA HA'.
+  Qed.
+
+  (* Lemma expand_failure_dead *)
+
+  Lemma succes_is_solved s {A}: valid_state A -> success A -> exists B, expand s A = Solved s B.
+  Proof.
+    elim: A s => //; try by do 2 eexists.
+    + move=> A HA s1 B HB s /simpl_valid_state_or[].
+        move=>[-> vB]/=.
+        rewrite dead_dead_same eqxx.
+        move=>sB.
+        by have [B' H] := HB s vB sB; rewrite H; eexists.
+      move=>[dA[vA bB]]/=.
+      case:ifP => /eqP// _ sA.
+      by have [A' H] := HA s vA sA; rewrite H; eexists.
+    + move=> A HA B0 HB0 B HB s /simpl_valid_state_and[] VA VB /=/andP[SA SB].
+      have [A' H1]:= HA s VA SA; rewrite H1.
+      have [B' H2]:= HB s VB SB; rewrite H2.
+      by eexists.
+  Qed.
+
+  Lemma expand_solved_success {s1 A s2 B}: 
+    valid_state A -> expand s1 A = Solved s2 B -> success A /\ success B.
+  Proof.
+    elim: A s1 s2 B => //.
+    + by move=> /= ???? [] /[subst2].
+    + move=> ? [] //.
+    + move=> A HA s B HB s1 s2 C /simpl_valid_state_or[].
+        move=> [] -> vB/=.
+        rewrite dead_dead_same eqxx.
+        case X: expand => //=-[]*;subst => /=.
+        rewrite dead_dead_same eqxx.
+        apply: HB X => //.
+      move=> [dA[VA bB]] /simpl_expand_or_solved[].
+        move=>[A'[HA' ->]]/=.
+        have:= expand_not_dead VA HA' => /=.
+        do 2 case: ifP => /eqP //; try congruence.
+        move=> ???; apply: HA VA HA'.
+      move=> [B'[]]//.
+    + move=> A HA ? _ B HB s1 s2 C /simpl_valid_state_and[VA VB].
+      move=> /simpl_expand_and_solved [s3 [A' [B'[HA' [HB' ->]]]]]/=.
+      have:= HA _ _ _ VA HA' => -[] ->->.
+      by have:= HB _ _ _ VB HB' => -[] ->->.
+  Qed.
+
+  Lemma expand_solved_failed {s1 A s2 B}: 
+    valid_state A -> expand s1 A = Solved s2 B -> failed A = false /\ failed B = false.
+  Proof.
+    move=>/expand_solved_success H /H[].
+    by do 2 move=> /success_failed->.
+  Qed.
+
+  Lemma expand_failure_failed {s1 A B}:
+    valid_state A -> expand s1 A = Failure B -> failed A /\ failed B.
+  Proof.
+    elim: A s1 B; clear => //; try by move=> ? [] //.
+    + move=> A HA s1 B HB s2 C /simpl_valid_state_or[].
+        move=> [] ->/=; rewrite dead_dead_same eqxx.
+        case X: expand => //= /HB{}HB [] <-; move: X=>/HB[]->/=.
+        by rewrite dead_dead_same eqxx.
+      move=> [DA] [] /[dup] VA /HA{}HA/[dup]BB/base_or_base_or_ko_valid/HB{}HB/simpl_expand_or_fail [].
+        move=> [A' [+[HD]]] /[subst1] /= dA.
+        have /= dA' :=expand_not_dead VA HD.
+        do 2 case: ifP => /eqP//; try congruence.
+        move=> _ _.
+        apply: HA HD.
+      move=> [B'[dA[HB'->]]]; rewrite dA /=.
+      rewrite dead_dead_same eqxx.
+      by apply: HB HB'.
+    + move=> A HA B0 _ B HB s C/simpl_valid_state_and[VA VB].
+      move=> /simpl_expand_and_fail[].
+        move=> [A' [HA'->]]/=.
+        by have:= HA _ _ VA HA'=>-[]-> //->.
+      move=> [s' [A' [B' [HA' [HB' ->]]]]]/=.
+      have:= HB _ _ VB HB' => -[]->->.
+      have:= expand_solved_success VA HA' => -[] ->->.
+      by rewrite !orbT.
+  Qed. 
+
+
+  Lemma valid_state_expand {s A r}:
+    valid_state A -> expand s A = r -> valid_state (get_state r).
+  Proof.
+    elim: A s r => //; try by move=> s r // *; subst.
+    + by move=> ? [|?] ?? *;subst => //=; rewrite valid_state_big_or.
+    + move=> A IHA s B IHB s1 r /simpl_valid_state_or[].  
+        move=> []->VB/=; rewrite dead_dead_same eqxx.
+        case X: expand => *; subst => /= ; rewrite dead_dead_same eqxx;
+        by have:= IHB _ _ VB X.
+      move=> [dA [VA bB]].
+      case: r.
+      + move=> s2 C /simpl_expand_or_expanded [].
+          move=> [A'[_[HA' ->]]]/=.
+          rewrite (IHA _ _ VA HA') bB.
+          have /= dA':= expand_not_dead VA HA'.
+          case: ifP => // _.
+          by apply: base_or_base_or_ko_valid.
+        move=> [].
+          move=>[A'[_[HA' ->]]]/=.
+          have/=->:= IHA _ _ VA HA'.
+          rewrite (valid_state_cut (base_or_base_or_ko_valid bB)).
+          by move: bB => /orP[/base_or_base_or_ko_cut|/base_or_ko_cut]->; rewrite orbT if_same.
+        move=>[]//.
+      + move=> s2 C /simpl_expand_or_cut. 
+        move=> [s3[B'[dA'[HB]]]]//.
+      + move=> C /simpl_expand_or_fail [].
+          move=>[A'[_[HA'->]]]/=.
+          have /= dA':= expand_not_dead VA HA'.
+          by case: ifP => /eqP// _; rewrite bB (IHA _ _ VA HA').
+        move=>[B'[?]]//.
+      + move=> s2 C /simpl_expand_or_solved [].
+          move=> [A'[HA' ->]]/=.
+          have /= dA':= expand_not_dead VA HA'.
+          by case: ifP => /eqP//; rewrite bB (IHA _ _ VA HA').
+        move=> [B'[?]]//.
+    + move=> A HA B0 _ B HB s1 r /simpl_valid_state_and1[VA[VB[ssB0 bB0]]].
+      case: r.
+      + move=> s2 C => /simpl_expand_and_expanded [].
+          move=> [A'[HA' ->]]/=.
+          rewrite (HA _ _ VA HA') bB0 (valid_state_compose_and VB bB0) ssB0.
+          move: VB.
+          case: ifP => //sA.
+          have:= succes_is_solved s1 VA sA; rewrite HA' => -[?] //.
+          by move=>->; rewrite if_same.
+        move=> [s[A'[B'[HA'[HB' ->]]]]]/=.
+        have:= expand_solved_success VA HA' => -[] _ ->.
+        rewrite (HA _ _ VA HA') (HB _ _ (valid_state_compose_and VB bB0) HB') bB0.
+        by rewrite (ssa_expand bB0 ssB0 HB').
+      + move=> s2 C /simpl_expand_and_cut [].
+          move=> [A' [HA' ->]]/=.
+          rewrite (HA _ _ VA HA') bB0 (valid_state_compose_and VB bB0).
+          move: VB; case SA: success.
+            have:= succes_is_solved s1 VA SA; rewrite HA' => -[?] //.
+          by move=>->; rewrite if_same ssB0.
+        move=> [s'[A'[B'[HA'[HB' ->]]]]]/=.
+        move: VB.
+        have:= expand_solved_success VA HA' => -[] -> sA' VB.
+        rewrite (HB _ _ VB HB') success_cut bB0 sA' (valid_state_cut (HA _ _ VA HA')).
+        by rewrite (ssa_expand bB0 ssB0 HB').
+      + move=> s2 /simpl_expand_and_fail [].
+          move=>[A'[HA'->]]/=.
+          rewrite (HA _ _ VA HA') bB0 ssB0.
+          have []:= expand_failure_failed VA HA'.
+          move: VB; case: ifP => //sA ->.
+            by move=> /failed_success; rewrite sA.
+          case: ifP => //.
+          by move=>/success_failed ->.
+        move=> [s'[A'[B'[HA'[HB' ->]]]]]/=.
+        have:= HA _ _ VA HA'.
+        have:= HB _ _ (valid_state_compose_and VB bB0) HB' => /=.
+        move=>->->.
+        have:= expand_solved_success VA HA' => -[] _ ->.
+        by rewrite (ssa_expand bB0 ssB0 HB') bB0.
+      + move=> s C /simpl_expand_and_solved [s'[A'[B'[HA' [HB'->]]]]]/=.
+        move: VB.
+        have:= expand_solved_success VA HA' => -[]->-> VB.
+        rewrite (HA _ _ VA HA') (HB _ _ VB HB') bB0.
+        by rewrite (ssa_expand bB0 ssB0 HB').
+  Qed.
+
+  Lemma valid_state_big_or_aux {pr s l} : valid_state (big_or_aux pr s l).
+  Proof.
+    elim: l s => [|[]] //=.
+    + move=> s; rewrite valid_state_big_and // full_expanded_big_and.
+    + move=> _ r l IH s.
+      by rewrite valid_state_big_and base_or_big_or_aux IH /= if_same.
+  Qed.
+
+  Lemma toT {P}: P = true -> is_true P.
+  Proof. case: P => //. Qed.
+
+  Definition get_state_run r := match r with Done _ s => s | Failed s => s end.
+
+  Lemma expandedP_expanded {s A r}:
+    valid_state A -> expanded s A r -> valid_state (get_state_run r).
+  Proof.
+    move=> + [b H]; elim H; clear.
+    + move=> s1 s2 A1 A2 EA VA /=.
+      apply: valid_state_expand VA EA.
+    + move=> s A B HA HB /=.
+      apply: valid_state_expand HB HA.
+    + move=> s s' r A B b HA HB IH VA.
+      have VB:= valid_state_expand VA HA.
+      apply: IH VB.
+    + move=> s s' r A B b HA HB IH VA.
+      have VB:= valid_state_expand VA HA.
+      apply: (IH VB).
+  Qed.
+
+  Lemma valid_state_expanded {s1 A r}:
+    valid_state A ->  expanded s1 A r -> valid_state (get_state_run r).
+  Proof.
+    move=> + [b H].
+    elim: H; clear.
+    + move=> s1 s2 A B HA VA /=; apply: valid_state_expand VA HA.
+    + move=> s A B HA VA; apply: valid_state_expand VA HA.
+    + move=> s1 s2 r A B b HA _ IH VA; apply (IH (valid_state_expand VA HA)).
+    + move=> s1 s2 r A B b HA _ IH VA; apply (IH (valid_state_expand VA HA)).
+  Qed.
+
+  Lemma next_alt_aux_base_and {s1 s2 A B}:
+     base_and A || base_and_ko A ->  next_alt_aux true s1 A = Some (s2, B) -> A = B.
+  Proof.
+    elim: A s1 s2 B => //; move=> [] //.
+    + move=> _ B0 _ B HB s1 s2 C /= /and3P[] bB0 /eqP cB0 bcB0.
+      case NB: next_alt_aux => // [[ ]] [] /[subst2].
+      by have:= HB _ _ _ _ NB; rewrite bcB0 orbT => /(_ isT) <-.
+    + move=> p a _ B0 HB0 B HB s1 s2 C /= /orP []// /andP []/eqP/[subst1] BB.
+      case NB: next_alt_aux => // [[ ]] [] /[subst2].
+      by rewrite BB in HB; rewrite (HB _ _ _ isT NB).
+  Qed.
+
+  Lemma next_alt_aux_base_and1 {s1 s2 A B}:
+     base_and A ->  next_alt_aux true s1 A = Some (s2, B) -> A = B.
+  Proof.
+    elim: A s1 s2 B => //; move=> [] //.
+    + move=> p a _ B0 HB0 B HB s1 s2 C /= /andP []/eqP/[subst1] BB.
+      case NB: next_alt_aux => // [[ ]] [] /[subst2].
+      by rewrite BB in HB; rewrite (HB _ _ _ isT NB).
+  Qed.
+
+  Lemma next_alt_aux_base_and2 {s1 s2 A B}:
+     base_and A ->  next_alt_aux true s1 (cut A) = Some (s2, B) -> cut A = B.
+  Proof.
+    elim: A s1 s2 B => //; move=> [] //.
+    + move=> p a _ B0 HB0 B HB s1 s2 C /= /andP []/eqP/[subst1] BB.
+      case NB: next_alt_aux => // [[ ]] [] /[subst2].
+      by rewrite BB in HB; rewrite (HB _ _ _ isT NB).
+  Qed.
+
+  (* Lemma xx {A B s}:
+    base_and A ->ssa A B -> 
+      exists s', next_alt_aux false s B = Some (s', A).
+  Proof.
+    elim: A B s => //.
+      move=>/= []//=. *)
+
+
+  Lemma ssa_next_alt_aux {B0 B s1 s2 D b}: 
+    base_and B0 -> ssa B0 B -> valid_state B ->
+      (* valid_state B -> *)
+        next_alt_aux b s1 B = Some (s2, D) -> ssa B0 D.
+  Proof.
+    elim: B0 B s1 s2 D b => //.
+      by move=> []//= s1 s2 D []// _ _ _ []??;subst.
+    move=>[]//p A IGN /= B0 HB0 B HB.
+    move=>[]// A' B0' B' s1 s2 D b.
+    move=>/andP[/eqP? bB]; subst => ssaB/=.
+    move=>/and3P[VA' VB']/andP[ssB0 bB0].
+    case NB' : (next_alt_aux true s1 B') => [[s3 E]|].
+      move=>[]??;subst.
+      rewrite (HB _ _ _ _ _ bB ssaB (valid_state_compose_and VB' bB0) NB')//.
+      (* by rewrite (HB _ _ _ _ _ bB _ ssaB NB')./ *)
+    case NA' : (next_alt_aux true s1 A') => // [[s3 E]].
+    move=>[]??;subst.
+    move: VB'.
+    case: ifP.
+      move=> H1 H2.
+      apply: xxx ssaB ssB0 => //.
+      (* admit. *)
+    move=> _.
+    move=>/orP[]/eqP?;subst => //.
+    apply: ssa_cut2 => //.
+  Qed.
+
+  Lemma valid_state_next_alt_aux {b s1 s2 A B}: 
+    valid_state A -> next_alt_aux b s1 A = Some (s2, B) 
+    -> valid_state B.
+  Proof.
+    elim: A b s1 s2 B => //.
+    + by move=> [] // ??? _ [] /[subst2].
+    + by move=> [] // ??? _ [] /[subst2].
+    + by move=> ?? [] // ??? _ [] /[subst2].
+    + move=> A HA s B HB b s1 s2 C /simpl_valid_state_or [].
+        move=> [-> VB]/=; rewrite dead_dead_same eqxx.
+        case X: next_alt_aux => // [[s3 D]].
+        case: ifP => ///eqP dD []*; subst => /=.
+        rewrite dead_dead_same eqxx; apply: HB VB X.
+      move=> [dA [VA bB]].
+      move=> /simpl_next_alt_aux_some [].
+        move=>[B'[?]]//.
+      move=> [_ [dB []]].
+        move=>[A'[NA->]]/=.
+        by rewrite bB (base_or_base_or_ko_valid)// (HA _ _ _ _ VA NA) if_same.
+      by move=>[NA->]/=; rewrite dead_dead_same eqxx (base_or_base_or_ko_valid bB).
+    + move=> A HA B0 HB0 B HB b s1 s2 C /simpl_valid_state_and1 [VA [VB [ssaB0 bB0]]]/=.
+      case NB: next_alt_aux => [[s3 D]|].
+        move=> [] /[subst2] /=; rewrite VA bB0.
+        move: VB.
+        case: ifP => SA//.
+          move=>VB; rewrite (HB _ _ _ _ VB NB) (ssa_next_alt_aux bB0 _ _ NB)//.
+        move=>/orP[]/eqP?;subst.
+          have <- := next_alt_aux_base_and1 bB0 NB.
+          by rewrite eqxx ssa_id//=.
+        have <- := next_alt_aux_base_and2 bB0 NB.
+        by rewrite eqxx orbT ssaB0.
+      case NA: next_alt_aux => // [[s3 D]] [] /[subst2] /=.
+      by rewrite (HA _ _ _ _ VA NA) eqxx bB0 (base_and_valid bB0) if_same ssa_id.
+  Qed.
+
+  Lemma valid_state_next_alt {s s' A B} : 
+    next_alt s A (Some (s', B)) -> valid_state A ->  valid_state B.
+  Proof.
+    remember (Some _) as S eqn:HS.
+    move=> H; elim: H s' B HS => //; clear.
+    + move=> s s2 A B' + FA s1 B [] /[subst2].
+      by move=> /valid_state_next_alt_aux H1.
+    + move=> s s1 r A B NA FB NB IH s2 D /[subst1] VA.
+      have VB:= valid_state_next_alt_aux VA NA.
+      apply: IH erefl VB.
+  Qed.
+
+  Lemma runP_run {s A r}:
+    valid_state A -> run s A r -> valid_state (get_state_run r).
+  Proof.
+    move=> + [b H]; elim H; clear.
+    + move=> s1 s2 A B b EA VA.
+      have H := valid_state_expanded VA (ex_intro _ _ EA).
+      exact H.
+    + move=> s A B b HA HB VA.
+      apply: valid_state_expanded VA (ex_intro _ _ HA).
+    + move=> s s' r A B C b1 b2 b3 HA HB HC IH Hb VA.
+      have VB := valid_state_expanded VA (ex_intro _ _ HA).
+      have NA := valid_state_next_alt HB VB.
+      apply: IH NA.
+    Qed.
+
+End valid_state.
